<?xml version="1.0"?>
<rdf:RDF xmlns="http://uk.gov.dstl/cis/d3#"
     xml:base="http://uk.gov.dstl/cis/d3"
     xmlns:d31="http://uk.gov.dstl/cis/d3/"
     xmlns:rdf="http://www.w3.org/1999/02/22-rdf-syntax-ns#"
     xmlns:baleen="http://baleen.dstl.gov.uk/"
     xmlns:owl="http://www.w3.org/2002/07/owl#"
     xmlns:xml="http://www.w3.org/XML/1998/namespace"
     xmlns:xsd="http://www.w3.org/2001/XMLSchema#"
     xmlns:rdfs="http://www.w3.org/2000/01/rdf-schema#"
     xmlns:demo="http://uk.gov.dstl/cis/d3/demo#"
     xmlns:sws="http://sws.geonames.org/"
     xmlns:dc="http://purl.org/dc/elements/1.1/"
     xmlns:d3="http://uk.gov.dstl/cis/d3#">
    <owl:Ontology/>
    


    <!-- 
    ///////////////////////////////////////////////////////////////////////////////////////
    //
    // Object Properties
    //
    ///////////////////////////////////////////////////////////////////////////////////////
     -->

    


    <!-- http://baleen.dstl.gov.uk/Relation -->

    <owl:ObjectProperty rdf:about="http://baleen.dstl.gov.uk/Relation">
        <rdfs:domain rdf:resource="http://baleen.dstl.gov.uk/Entity"/>
        <rdfs:range rdf:resource="http://baleen.dstl.gov.uk/Entity"/>
    </owl:ObjectProperty>
    


    <!-- http://baleen.dstl.gov.uk/mentionIn -->

    <owl:ObjectProperty rdf:about="http://baleen.dstl.gov.uk/mentionIn">
        <rdfs:domain rdf:resource="http://baleen.dstl.gov.uk/Mention"/>
        <rdfs:range rdf:resource="http://baleen.dstl.gov.uk/Document"/>
        <rdfs:comment xml:lang="en">The document this is mentioned in</rdfs:comment>
    </owl:ObjectProperty>
    


    <!-- http://baleen.dstl.gov.uk/mentionOf -->

    <owl:ObjectProperty rdf:about="http://baleen.dstl.gov.uk/mentionOf">
        <rdfs:domain rdf:resource="http://baleen.dstl.gov.uk/Entity"/>
        <rdfs:range rdf:resource="http://baleen.dstl.gov.uk/ReferenceTarget"/>
        <rdfs:comment xml:lang="en">The mention of the reference</rdfs:comment>
    </owl:ObjectProperty>
    


    <!-- http://baleen.dstl.gov.uk/participantIn -->

    <owl:ObjectProperty rdf:about="http://baleen.dstl.gov.uk/participantIn">
        <rdfs:domain rdf:resource="http://baleen.dstl.gov.uk/Entity"/>
        <rdfs:range rdf:resource="http://baleen.dstl.gov.uk/Event"/>
        <rdfs:comment xml:lang="en">A participant in the event</rdfs:comment>
    </owl:ObjectProperty>
    


    <!-- http://baleen.dstl.gov.uk/source -->

    <owl:ObjectProperty rdf:about="http://baleen.dstl.gov.uk/source">
        <rdfs:domain rdf:resource="http://baleen.dstl.gov.uk/Entity"/>
        <rdfs:range rdf:resource="http://baleen.dstl.gov.uk/Relation"/>
    </owl:ObjectProperty>
    


    <!-- http://baleen.dstl.gov.uk/target -->

    <owl:ObjectProperty rdf:about="http://baleen.dstl.gov.uk/target">
        <rdfs:domain rdf:resource="http://baleen.dstl.gov.uk/Relation"/>
        <rdfs:range rdf:resource="http://baleen.dstl.gov.uk/Entity"/>
    </owl:ObjectProperty>
    


    <!-- 
    ///////////////////////////////////////////////////////////////////////////////////////
    //
    // Data properties
    //
    ///////////////////////////////////////////////////////////////////////////////////////
     -->

    


    <!-- http://baleen.dstl.gov.uk/amount -->

    <owl:DatatypeProperty rdf:about="http://baleen.dstl.gov.uk/amount">
        <rdfs:domain rdf:resource="http://baleen.dstl.gov.uk/Money"/>
        <rdfs:range rdf:resource="http://www.w3.org/2001/XMLSchema#double"/>
        <rdfs:comment xml:lang="en">Numeric value of amount of money mentioned in document.</rdfs:comment>
    </owl:DatatypeProperty>
    


    <!-- http://baleen.dstl.gov.uk/arguments -->

    <owl:DatatypeProperty rdf:about="http://baleen.dstl.gov.uk/arguments">
        <rdfs:domain rdf:resource="http://baleen.dstl.gov.uk/Event"/>
        <rdfs:range rdf:resource="http://www.w3.org/2001/XMLSchema#string"/>
        <rdfs:comment xml:lang="en">Additional text information, such as subject/object, in addition to the entities.</rdfs:comment>
    </owl:DatatypeProperty>
    


    <!-- http://baleen.dstl.gov.uk/begin -->

    <owl:DatatypeProperty rdf:about="http://baleen.dstl.gov.uk/begin">
        <rdfs:domain rdf:resource="http://baleen.dstl.gov.uk/Mention"/>
        <rdfs:range rdf:resource="http://www.w3.org/2001/XMLSchema#int"/>
        <rdfs:comment xml:lang="en">The start of the mention offset</rdfs:comment>
    </owl:DatatypeProperty>
    


    <!-- http://baleen.dstl.gov.uk/confidence -->

    <owl:DatatypeProperty rdf:about="http://baleen.dstl.gov.uk/confidence">
        <rdfs:domain rdf:resource="http://baleen.dstl.gov.uk/Document"/>
        <rdfs:range rdf:resource="http://www.w3.org/2001/XMLSchema#double"/>
        <rdfs:comment xml:lang="en">Confidence value between 0 and 1 from annotation processor.</rdfs:comment>
    </owl:DatatypeProperty>
    


    <!-- http://baleen.dstl.gov.uk/coordinateValue -->

    <owl:DatatypeProperty rdf:about="http://baleen.dstl.gov.uk/coordinateValue">
        <rdfs:domain rdf:resource="http://baleen.dstl.gov.uk/Coordinate"/>
        <rdfs:range rdf:resource="http://www.w3.org/2001/XMLSchema#string"/>
        <rdfs:comment xml:lang="en">A normalised value for the coordinate.</rdfs:comment>
    </owl:DatatypeProperty>
    


    <!-- http://baleen.dstl.gov.uk/countryCode -->

    <owl:DatatypeProperty rdf:about="http://baleen.dstl.gov.uk/countryCode">
        <rdfs:domain rdf:resource="http://baleen.dstl.gov.uk/Nationality"/>
        <rdfs:range rdf:resource="http://www.w3.org/2001/XMLSchema#string"/>
        <rdfs:comment xml:lang="en">The country code associated with this nationality, e.g. FRA for French</rdfs:comment>
    </owl:DatatypeProperty>
    


    <!-- http://baleen.dstl.gov.uk/currency -->

    <owl:DatatypeProperty rdf:about="http://baleen.dstl.gov.uk/currency">
        <rdfs:domain rdf:resource="http://baleen.dstl.gov.uk/Money"/>
        <rdfs:range rdf:resource="http://www.w3.org/2001/XMLSchema#string"/>
        <rdfs:comment xml:lang="en">String value of the currency denomination the money amount is specified in.</rdfs:comment>
    </owl:DatatypeProperty>
    


    <!-- http://baleen.dstl.gov.uk/dependencyDistance -->

    <owl:DatatypeProperty rdf:about="http://baleen.dstl.gov.uk/dependencyDistance">
        <rdfs:domain rdf:resource="http://baleen.dstl.gov.uk/Relation"/>
        <rdfs:range rdf:resource="http://www.w3.org/2001/XMLSchema#int"/>
        <rdfs:comment xml:lang="en">A measure of the dependency distance in the sentence between the two entities. The number of dependant words between the two entities according to a dependency parser.</rdfs:comment>
    </owl:DatatypeProperty>
    


    <!-- http://baleen.dstl.gov.uk/depth -->

    <owl:DatatypeProperty rdf:about="http://baleen.dstl.gov.uk/depth">
        <rdfs:domain rdf:resource="http://baleen.dstl.gov.uk/Document"/>
        <rdfs:range rdf:resource="http://www.w3.org/2001/XMLSchema#int"/>
        <rdfs:comment xml:lang="en">The depth of the structural component.</rdfs:comment>
    </owl:DatatypeProperty>
    


    <!-- http://baleen.dstl.gov.uk/docId -->

    <owl:DatatypeProperty rdf:about="http://baleen.dstl.gov.uk/docId">
        <rdfs:domain rdf:resource="http://baleen.dstl.gov.uk/Mention"/>
        <rdfs:range rdf:resource="http://www.w3.org/2001/XMLSchema#string"/>
        <rdfs:comment xml:lang="en">The docId the mention came from</rdfs:comment>
    </owl:DatatypeProperty>
    


    <!-- http://baleen.dstl.gov.uk/elementClass -->

    <owl:DatatypeProperty rdf:about="http://baleen.dstl.gov.uk/elementClass">
        <rdfs:domain rdf:resource="http://baleen.dstl.gov.uk/Document"/>
        <rdfs:range rdf:resource="http://www.w3.org/2001/XMLSchema#string"/>
        <rdfs:comment xml:lang="en">A holder for further class information, say a more specific html class or a defined word style.</rdfs:comment>
    </owl:DatatypeProperty>
    


    <!-- http://baleen.dstl.gov.uk/elementId -->

    <owl:DatatypeProperty rdf:about="http://baleen.dstl.gov.uk/elementId">
        <rdfs:domain rdf:resource="http://baleen.dstl.gov.uk/Document"/>
        <rdfs:range rdf:resource="http://www.w3.org/2001/XMLSchema#string"/>
        <rdfs:comment xml:lang="en">A holder for an id, if defined from the format.</rdfs:comment>
    </owl:DatatypeProperty>
    


    <!-- http://baleen.dstl.gov.uk/end -->

    <owl:DatatypeProperty rdf:about="http://baleen.dstl.gov.uk/end">
        <rdfs:domain rdf:resource="http://baleen.dstl.gov.uk/Mention"/>
        <rdfs:range rdf:resource="http://www.w3.org/2001/XMLSchema#int"/>
        <rdfs:comment xml:lang="en">The end of the mention offset</rdfs:comment>
    </owl:DatatypeProperty>
    


    <!-- http://baleen.dstl.gov.uk/entities -->

    <owl:DatatypeProperty rdf:about="http://baleen.dstl.gov.uk/entities">
        <rdfs:domain rdf:resource="http://baleen.dstl.gov.uk/Event"/>
        <rdfs:range rdf:resource="http://www.w3.org/2001/XMLSchema#string"/>
        <rdfs:comment xml:lang="en">The entities which are involved / related / associated with the event.</rdfs:comment>
    </owl:DatatypeProperty>
    


    <!-- http://baleen.dstl.gov.uk/eventType -->

    <owl:DatatypeProperty rdf:about="http://baleen.dstl.gov.uk/eventType">
        <rdfs:domain rdf:resource="http://baleen.dstl.gov.uk/Event"/>
        <rdfs:range rdf:resource="http://www.w3.org/2001/XMLSchema#string"/>
        <rdfs:comment xml:lang="en">The event type which classifies the event.

For example Currently based on the ACE2002 top-level relationships: {&quot;AT&quot; , &quot;NEAR&quot; , &quot;PART&quot; , &quot;ROLE&quot; , &quot;SOCIAL&quot;}
Additional relationship types that have been added: {&quot;QUANTITY&quot;, &quot;ALIAS&quot;}</rdfs:comment>
    </owl:DatatypeProperty>
    


    <!-- http://baleen.dstl.gov.uk/gender -->

    <owl:DatatypeProperty rdf:about="http://baleen.dstl.gov.uk/gender">
        <rdfs:domain rdf:resource="http://baleen.dstl.gov.uk/Person"/>
        <rdfs:range rdf:resource="http://www.w3.org/2001/XMLSchema#string"/>
        <rdfs:comment xml:lang="en">Should be one of the following:
* MALE
* FEMALE
* UNKNOWN

If empty or null, it is assumed to be UNKNOWN.</rdfs:comment>
    </owl:DatatypeProperty>
    


    <!-- http://baleen.dstl.gov.uk/geoJson -->

    <owl:DatatypeProperty rdf:about="http://baleen.dstl.gov.uk/geoJson">
        <rdfs:domain rdf:resource="http://baleen.dstl.gov.uk/Location"/>
        <rdfs:range rdf:resource="http://www.w3.org/2001/XMLSchema#string"/>
        <rdfs:comment xml:lang="en">A strnig representation of geoJson format represention of geographic information associated with the location, including where possible coordinate(s).</rdfs:comment>
    </owl:DatatypeProperty>
    


    <!-- http://baleen.dstl.gov.uk/isNormalised -->

    <owl:DatatypeProperty rdf:about="http://baleen.dstl.gov.uk/isNormalised">
        <rdfs:domain rdf:resource="http://baleen.dstl.gov.uk/Entity"/>
        <rdfs:range rdf:resource="http://www.w3.org/2001/XMLSchema#boolean"/>
        <rdfs:comment xml:lang="en">Marks the entity value as having been normalised from the original value</rdfs:comment>
    </owl:DatatypeProperty>
    


    <!-- http://baleen.dstl.gov.uk/linking -->

    <owl:DatatypeProperty rdf:about="http://baleen.dstl.gov.uk/linking">
        <rdfs:domain rdf:resource="http://baleen.dstl.gov.uk/ReferenceTarget"/>
        <rdfs:range rdf:resource="http://www.w3.org/2001/XMLSchema#string"/>
        <rdfs:comment xml:lang="en">A property to define an external linking that may describe this group of mentions. For example, a set of mentions of a person could be linked to a database entry or webpage for the person.</rdfs:comment>
    </owl:DatatypeProperty>
    


    <!-- http://baleen.dstl.gov.uk/normalizedQuantity -->

    <owl:DatatypeProperty rdf:about="http://baleen.dstl.gov.uk/normalizedQuantity">
        <rdfs:domain rdf:resource="http://baleen.dstl.gov.uk/Quantity"/>
        <rdfs:range rdf:resource="http://www.w3.org/2001/XMLSchema#double"/>
        <rdfs:comment xml:lang="en">The normalized quantity</rdfs:comment>
    </owl:DatatypeProperty>
    


    <!-- http://baleen.dstl.gov.uk/normalizedUnit -->

    <owl:DatatypeProperty rdf:about="http://baleen.dstl.gov.uk/normalizedUnit">
        <rdfs:domain rdf:resource="http://baleen.dstl.gov.uk/Quantity"/>
        <rdfs:range rdf:resource="http://www.w3.org/2001/XMLSchema#string"/>
        <rdfs:comment xml:lang="en">The unit of the normalized quantity</rdfs:comment>
    </owl:DatatypeProperty>
    


    <!-- http://baleen.dstl.gov.uk/precision -->

    <owl:DatatypeProperty rdf:about="http://baleen.dstl.gov.uk/precision">
        <rdfs:domain rdf:resource="http://baleen.dstl.gov.uk/Temporal"/>
        <rdfs:range rdf:resource="http://www.w3.org/2001/XMLSchema#string"/>
        <rdfs:comment xml:lang="en">What level of precision does this temporal entity have. Do we know exactly when it refers to (i.e. we would expect to know timestampStart and timestampEnd); or is it relative to something else (i.e. we would expect to know timestampStart and timestampEnd only if we know when it is relative to); or is it unqualified (i.e. we would not expect to know timestampStart and timestampStop)?

If unknown, then leave as null (or empty).

Expected values: EXACT, RELATIVE, UNQUALIFIED, null</rdfs:comment>
    </owl:DatatypeProperty>
    


    <!-- http://baleen.dstl.gov.uk/quantity -->

    <owl:DatatypeProperty rdf:about="http://baleen.dstl.gov.uk/quantity">
        <rdfs:domain rdf:resource="http://baleen.dstl.gov.uk/Quantity"/>
        <rdfs:range rdf:resource="http://www.w3.org/2001/XMLSchema#double"/>
        <rdfs:comment xml:lang="en">The raw quantity</rdfs:comment>
    </owl:DatatypeProperty>
    


    <!-- http://baleen.dstl.gov.uk/referent -->

    <owl:DatatypeProperty rdf:about="http://baleen.dstl.gov.uk/referent">
        <rdfs:domain rdf:resource="http://baleen.dstl.gov.uk/Document"/>
        <rdfs:range rdf:resource="http://www.w3.org/2001/XMLSchema#string"/>
        <rdfs:comment xml:lang="en">Can be used to link a corefence to an entity to another (presuambly more definitive) mention of the same entity elsewhere in the text.</rdfs:comment>
    </owl:DatatypeProperty>
    


    <!-- http://baleen.dstl.gov.uk/relationSubType -->

    <owl:DatatypeProperty rdf:about="http://baleen.dstl.gov.uk/relationSubType">
        <rdfs:domain rdf:resource="http://baleen.dstl.gov.uk/Relation"/>
        <rdfs:range rdf:resource="http://www.w3.org/2001/XMLSchema#string"/>
        <rdfs:comment xml:lang="en">Used to record any sub-type information for the relation, for example the sub-relations defined within the ACE dataset.</rdfs:comment>
    </owl:DatatypeProperty>
    


    <!-- http://baleen.dstl.gov.uk/relationshipType -->

    <owl:DatatypeProperty rdf:about="http://baleen.dstl.gov.uk/relationshipType">
        <rdfs:domain rdf:resource="http://baleen.dstl.gov.uk/Relation"/>
        <rdfs:range rdf:resource="http://www.w3.org/2001/XMLSchema#string"/>
        <rdfs:comment xml:lang="en">Denotes the semantic type of the relationship between entities. 

Currently based on the ACE2002 top-level relationships: {&quot;AT&quot; , &quot;NEAR&quot; , &quot;PART&quot; , &quot;ROLE&quot; , &quot;SOCIAL&quot;}
Additional relationship types that have been added: {&quot;QUANTITY&quot;, &quot;ALIAS&quot;}</rdfs:comment>
    </owl:DatatypeProperty>
    


    <!-- http://baleen.dstl.gov.uk/scope -->

    <owl:DatatypeProperty rdf:about="http://baleen.dstl.gov.uk/scope">
        <rdfs:domain rdf:resource="http://baleen.dstl.gov.uk/Temporal"/>
        <rdfs:range rdf:resource="http://www.w3.org/2001/XMLSchema#string"/>
        <rdfs:comment xml:lang="en">Does this temporal entity describe a single temporal instance (e.g. 12 Oct 2016) or a temporal range (12-16 Oct 2016). If unknown, then leave as null (or empty).

Expected values: SINGLE, RANGE, null</rdfs:comment>
    </owl:DatatypeProperty>
    


    <!-- http://baleen.dstl.gov.uk/sentenceDistance -->

    <owl:DatatypeProperty rdf:about="http://baleen.dstl.gov.uk/sentenceDistance">
        <rdfs:domain rdf:resource="http://baleen.dstl.gov.uk/Relation"/>
        <rdfs:range rdf:resource="http://www.w3.org/2001/XMLSchema#int"/>
        <rdfs:comment xml:lang="en">A measure of the distance in the document between the two entities. The number of sentences between the two entities.</rdfs:comment>
    </owl:DatatypeProperty>
    


    <!-- http://baleen.dstl.gov.uk/source -->

    <owl:DatatypeProperty rdf:about="http://baleen.dstl.gov.uk/source"/>
    


    <!-- http://baleen.dstl.gov.uk/subType -->

    <owl:DatatypeProperty rdf:about="http://baleen.dstl.gov.uk/subType">
        <rdfs:domain rdf:resource="http://baleen.dstl.gov.uk/Entity"/>
        <rdfs:range rdf:resource="http://www.w3.org/2001/XMLSchema#string"/>
        <rdfs:comment xml:lang="en">String identifying sub type of entity.</rdfs:comment>
    </owl:DatatypeProperty>
    


    <!-- http://baleen.dstl.gov.uk/tags -->

    <owl:DatatypeProperty rdf:about="http://baleen.dstl.gov.uk/tags">
        <rdfs:domain rdf:resource="http://baleen.dstl.gov.uk/Buzzword"/>
        <rdfs:range rdf:resource="http://www.w3.org/2001/XMLSchema#string"/>
        <rdfs:comment xml:lang="en">A list of types that are associated with a given BuzzWord value.</rdfs:comment>
    </owl:DatatypeProperty>
    


    <!-- http://baleen.dstl.gov.uk/target -->

    <owl:DatatypeProperty rdf:about="http://baleen.dstl.gov.uk/target"/>
    


    <!-- http://baleen.dstl.gov.uk/temporalType -->

    <owl:DatatypeProperty rdf:about="http://baleen.dstl.gov.uk/temporalType">
        <rdfs:domain rdf:resource="http://baleen.dstl.gov.uk/Temporal"/>
        <rdfs:range rdf:resource="http://www.w3.org/2001/XMLSchema#string"/>
        <rdfs:comment xml:lang="en">Does this temporal entity describe a date, a time or a datetime. If unknown, then leave as null (or empty).

Expected values: DATE, TIME, DATETIME, null</rdfs:comment>
    </owl:DatatypeProperty>
    


    <!-- http://baleen.dstl.gov.uk/timestampStart -->

    <owl:DatatypeProperty rdf:about="http://baleen.dstl.gov.uk/timestampStart">
        <rdfs:domain rdf:resource="http://baleen.dstl.gov.uk/Temporal"/>
        <rdfs:range rdf:resource="http://www.w3.org/2001/XMLSchema#long"/>
        <rdfs:comment xml:lang="en">Timestamp of the point when the temporal reference starts (inclusive), in seconds.</rdfs:comment>
    </owl:DatatypeProperty>
    


    <!-- http://baleen.dstl.gov.uk/timestampStop -->

    <owl:DatatypeProperty rdf:about="http://baleen.dstl.gov.uk/timestampStop">
        <rdfs:domain rdf:resource="http://baleen.dstl.gov.uk/Temporal"/>
        <rdfs:range rdf:resource="http://www.w3.org/2001/XMLSchema#long"/>
        <rdfs:comment xml:lang="en">Timestamp of the point when the temporal reference ends (exclusive), in seconds.</rdfs:comment>
    </owl:DatatypeProperty>
    


    <!-- http://baleen.dstl.gov.uk/title -->

    <owl:DatatypeProperty rdf:about="http://baleen.dstl.gov.uk/title">
        <rdfs:domain rdf:resource="http://baleen.dstl.gov.uk/Person"/>
        <rdfs:range rdf:resource="http://www.w3.org/2001/XMLSchema#string"/>
        <rdfs:comment xml:lang="en">A person&apos;s title, for example Mr or President</rdfs:comment>
    </owl:DatatypeProperty>
    


    <!-- http://baleen.dstl.gov.uk/tokens -->

    <owl:DatatypeProperty rdf:about="http://baleen.dstl.gov.uk/tokens">
        <rdfs:domain rdf:resource="http://baleen.dstl.gov.uk/Event"/>
        <rdfs:range rdf:resource="http://www.w3.org/2001/XMLSchema#string"/>
        <rdfs:comment xml:lang="en">WordTokens which relate to the event type (eg verbs in the sentence)</rdfs:comment>
    </owl:DatatypeProperty>
    


    <!-- http://baleen.dstl.gov.uk/unit -->

    <owl:DatatypeProperty rdf:about="http://baleen.dstl.gov.uk/unit">
        <rdfs:domain rdf:resource="http://baleen.dstl.gov.uk/Quantity"/>
        <rdfs:range rdf:resource="http://www.w3.org/2001/XMLSchema#string"/>
        <rdfs:comment xml:lang="en">The unit of the raw quantity</rdfs:comment>
    </owl:DatatypeProperty>
    


    <!-- http://baleen.dstl.gov.uk/value -->

    <owl:DatatypeProperty rdf:about="http://baleen.dstl.gov.uk/value">
        <rdfs:domain rdf:resource="http://baleen.dstl.gov.uk/Mention"/>
        <rdfs:range rdf:resource="http://www.w3.org/2001/XMLSchema#string"/>
        <rdfs:comment xml:lang="en">The value of the mention</rdfs:comment>
    </owl:DatatypeProperty>
    


    <!-- http://baleen.dstl.gov.uk/vehicleIdentifier -->

    <owl:DatatypeProperty rdf:about="http://baleen.dstl.gov.uk/vehicleIdentifier">
        <rdfs:domain rdf:resource="http://baleen.dstl.gov.uk/Vehicle"/>
        <rdfs:range rdf:resource="http://www.w3.org/2001/XMLSchema#string"/>
        <rdfs:comment xml:lang="en">An identifying name or number for the vehicle</rdfs:comment>
    </owl:DatatypeProperty>
    


    <!-- http://baleen.dstl.gov.uk/wordDistance -->

    <owl:DatatypeProperty rdf:about="http://baleen.dstl.gov.uk/wordDistance">
        <rdfs:domain rdf:resource="http://baleen.dstl.gov.uk/Relation"/>
        <rdfs:range rdf:resource="http://www.w3.org/2001/XMLSchema#int"/>
        <rdfs:comment xml:lang="en">A measure of the distance in the sentence between the two entities. The number of words between the two entities.</rdfs:comment>
    </owl:DatatypeProperty>
    


    <!-- 
    ///////////////////////////////////////////////////////////////////////////////////////
    //
    // Classes
    //
    ///////////////////////////////////////////////////////////////////////////////////////
     -->

    


    <!-- http://baleen.dstl.gov.uk/Buzzword -->

    <owl:Class rdf:about="http://baleen.dstl.gov.uk/Buzzword">
        <rdfs:subClassOf rdf:resource="http://baleen.dstl.gov.uk/Entity"/>
        <rdfs:comment xml:lang="en">User-defined key phrases or domain-specific terms, described by a type property.</rdfs:comment>
    </owl:Class>
    


    <!-- http://baleen.dstl.gov.uk/Chemical -->

    <owl:Class rdf:about="http://baleen.dstl.gov.uk/Chemical">
        <rdfs:subClassOf rdf:resource="http://baleen.dstl.gov.uk/Entity"/>
        <rdfs:comment xml:lang="en">A chemical or substance</rdfs:comment>
    </owl:Class>
    


    <!-- http://baleen.dstl.gov.uk/CommsIdentifier -->

    <owl:Class rdf:about="http://baleen.dstl.gov.uk/CommsIdentifier">
        <rdfs:subClassOf rdf:resource="http://baleen.dstl.gov.uk/Entity"/>
        <rdfs:comment xml:lang="en">A communication identifier - including equipent, user, accounts or subscription.  Includes (but not limited to) the following types: emailAddress, IPv4, IPv6, MSISDN, IMEI, IMSI values.</rdfs:comment>
    </owl:Class>
    


    <!-- http://baleen.dstl.gov.uk/Coordinate -->

    <owl:Class rdf:about="http://baleen.dstl.gov.uk/Coordinate">
        <rdfs:subClassOf rdf:resource="http://baleen.dstl.gov.uk/Location"/>
        <rdfs:comment xml:lang="en">A well-formed coordinate value - MGRS or WGS84 DD or DMS coordinate system - explicitly defined in source document.</rdfs:comment>
    </owl:Class>
    


    <!-- http://baleen.dstl.gov.uk/Document -->

    <owl:Class rdf:about="http://baleen.dstl.gov.uk/Document">
        <rdfs:comment xml:lang="en">A document.</rdfs:comment>
    </owl:Class>
    


    <!-- http://baleen.dstl.gov.uk/DocumentReference -->

    <owl:Class rdf:about="http://baleen.dstl.gov.uk/DocumentReference">
        <rdfs:subClassOf rdf:resource="http://baleen.dstl.gov.uk/Entity"/>
        <rdfs:comment xml:lang="en">A publication reference/serial/identifier within the source document.</rdfs:comment>
    </owl:Class>
    


    <!-- http://baleen.dstl.gov.uk/Entity -->

    <owl:Class rdf:about="http://baleen.dstl.gov.uk/Entity">
        <rdfs:subClassOf rdf:resource="http://baleen.dstl.gov.uk/Mention"/>
        <rdfs:comment xml:lang="en">Type to represent named entities - values that are assigned a semantic type.</rdfs:comment>
    </owl:Class>
    


    <!-- http://baleen.dstl.gov.uk/Event -->

    <owl:Class rdf:about="http://baleen.dstl.gov.uk/Event">
        <rdfs:subClassOf rdf:resource="http://baleen.dstl.gov.uk/Mention"/>
        <rdfs:comment xml:lang="en">An event relates one or more entities with an associated action.</rdfs:comment>
    </owl:Class>
    


    <!-- http://baleen.dstl.gov.uk/Frequency -->

    <owl:Class rdf:about="http://baleen.dstl.gov.uk/Frequency">
        <rdfs:subClassOf rdf:resource="http://baleen.dstl.gov.uk/Entity"/>
        <rdfs:comment xml:lang="en">A specific frequency value in the electro-magnetic spectrum (Hertz - Hz, MHz, GHz etc.).</rdfs:comment>
    </owl:Class>
    


    <!-- http://baleen.dstl.gov.uk/Location -->

    <owl:Class rdf:about="http://baleen.dstl.gov.uk/Location">
        <rdfs:subClassOf rdf:resource="http://baleen.dstl.gov.uk/Entity"/>
        <rdfs:comment xml:lang="en">A reference to a place, country, administrative region or geo-political entity within the source document. This is a general purpose type that is extended in &quot;geo&quot; types.</rdfs:comment>
    </owl:Class>
    


    <!-- http://baleen.dstl.gov.uk/Mention -->

    <owl:Class rdf:about="http://baleen.dstl.gov.uk/Mention">
        <rdfs:comment xml:lang="en">Root mention type</rdfs:comment>
    </owl:Class>
    


    <!-- http://baleen.dstl.gov.uk/MilitaryPlatform -->

    <owl:Class rdf:about="http://baleen.dstl.gov.uk/MilitaryPlatform">
        <rdfs:subClassOf rdf:resource="http://baleen.dstl.gov.uk/Entity"/>
        <rdfs:comment xml:lang="en">A reference to a military platform - space, air, land, surface and sub-surface platforms, where the type platform is described as a property.</rdfs:comment>
    </owl:Class>
    


    <!-- http://baleen.dstl.gov.uk/Money -->

    <owl:Class rdf:about="http://baleen.dstl.gov.uk/Money">
        <rdfs:subClassOf rdf:resource="http://baleen.dstl.gov.uk/Entity"/>
        <rdfs:comment xml:lang="en">Specific amount of some current mentioned within the document.</rdfs:comment>
    </owl:Class>
    


    <!-- http://baleen.dstl.gov.uk/Nationality -->

    <owl:Class rdf:about="http://baleen.dstl.gov.uk/Nationality">
        <rdfs:subClassOf rdf:resource="http://baleen.dstl.gov.uk/Entity"/>
        <rdfs:comment xml:lang="en">Nationality denonym (e.g. French, British, Spanish)</rdfs:comment>
    </owl:Class>
    


    <!-- http://baleen.dstl.gov.uk/Organisation -->

    <owl:Class rdf:about="http://baleen.dstl.gov.uk/Organisation">
        <rdfs:subClassOf rdf:resource="http://baleen.dstl.gov.uk/Entity"/>
        <rdfs:comment xml:lang="en">An explicit refrence to a formal organisation, including governmental, political, religious, charitable, economic/financial, business or criminal bodies.</rdfs:comment>
    </owl:Class>
    


    <!-- http://baleen.dstl.gov.uk/Person -->

    <owl:Class rdf:about="http://baleen.dstl.gov.uk/Person">
        <rdfs:subClassOf rdf:resource="http://baleen.dstl.gov.uk/Entity"/>
        <rdfs:comment xml:lang="en">A Person named entitiy, as defined by an explict name reference within the source document.</rdfs:comment>
    </owl:Class>
    


    <!-- http://baleen.dstl.gov.uk/Quantity -->

    <owl:Class rdf:about="http://baleen.dstl.gov.uk/Quantity">
        <rdfs:subClassOf rdf:resource="http://baleen.dstl.gov.uk/Entity"/>
        <rdfs:comment xml:lang="en">Type to annotate references to quantities within text</rdfs:comment>
    </owl:Class>
    


    <!-- http://baleen.dstl.gov.uk/ReferenceTarget -->

    <owl:Class rdf:about="http://baleen.dstl.gov.uk/ReferenceTarget">
        <rdfs:comment xml:lang="en">A target type for the referent property, such that entities pointing to the same target are assumed to be coreferences. The target can therefore be thought of as a super-entity, though it has no properties or value of it&apos;s own. The span of this entity is taken to be the scope in which this reference target is valid.</rdfs:comment>
    </owl:Class>
    


    <!-- http://baleen.dstl.gov.uk/Relation -->

    <owl:Class rdf:about="http://baleen.dstl.gov.uk/Relation">
        <rdfs:subClassOf rdf:resource="http://baleen.dstl.gov.uk/Mention"/>
    </owl:Class>
    


    <!-- http://baleen.dstl.gov.uk/SlideShow -->

    <owl:Class rdf:about="http://baleen.dstl.gov.uk/SlideShow">
        <rdfs:subClassOf rdf:resource="http://baleen.dstl.gov.uk/Document"/>
        <rdfs:comment xml:lang="en">A slide show.</rdfs:comment>
    </owl:Class>
    


    <!-- http://baleen.dstl.gov.uk/SpreadSheet -->

    <owl:Class rdf:about="http://baleen.dstl.gov.uk/SpreadSheet">
        <rdfs:subClassOf rdf:resource="http://baleen.dstl.gov.uk/Document"/>
        <rdfs:comment xml:lang="en">A spread sheet file.</rdfs:comment>
    </owl:Class>
    


    <!-- http://baleen.dstl.gov.uk/Temporal -->

    <owl:Class rdf:about="http://baleen.dstl.gov.uk/Temporal">
        <rdfs:subClassOf rdf:resource="http://baleen.dstl.gov.uk/Entity"/>
        <rdfs:comment xml:lang="en">Type to record all temporal references in the text and, where possible, information about them (e.g. timestamp). This includes all times, dates, datetimes, periods, etc.</rdfs:comment>
    </owl:Class>
    


    <!-- http://baleen.dstl.gov.uk/TextDocument -->

    <owl:Class rdf:about="http://baleen.dstl.gov.uk/TextDocument">
        <rdfs:subClassOf rdf:resource="http://baleen.dstl.gov.uk/Document"/>
        <rdfs:comment xml:lang="en">A text based document.</rdfs:comment>
    </owl:Class>
    


    <!-- http://baleen.dstl.gov.uk/Url -->

    <owl:Class rdf:about="http://baleen.dstl.gov.uk/Url">
        <rdfs:subClassOf rdf:resource="http://baleen.dstl.gov.uk/Entity"/>
        <rdfs:comment xml:lang="en">A well-formed uniform resource location (URL) value</rdfs:comment>
    </owl:Class>
    


    <!-- http://baleen.dstl.gov.uk/Vehicle -->

    <owl:Class rdf:about="http://baleen.dstl.gov.uk/Vehicle">
        <rdfs:subClassOf rdf:resource="http://baleen.dstl.gov.uk/Entity"/>
        <rdfs:comment xml:lang="en">Specific vehicle or vessel</rdfs:comment>
    </owl:Class>
    


    <!-- http://baleen.dstl.gov.uk/Vulnerability -->

    <owl:Class rdf:about="http://baleen.dstl.gov.uk/Vulnerability">
        <rdfs:subClassOf rdf:resource="http://baleen.dstl.gov.uk/Entity"/>
        <rdfs:comment xml:lang="en">Cyber vulnerabilities</rdfs:comment>
    </owl:Class>
    


    <!-- http://baleen.dstl.gov.uk/Weapon -->

    <owl:Class rdf:about="http://baleen.dstl.gov.uk/Weapon">
        <rdfs:subClassOf rdf:resource="http://baleen.dstl.gov.uk/Entity"/>
        <rdfs:comment xml:lang="en">A weapon; for example a rifle, knife, or shotgun</rdfs:comment>
    </owl:Class>
    


    <!-- 
    ///////////////////////////////////////////////////////////////////////////////////////
    //
    // Annotations
    //
    ///////////////////////////////////////////////////////////////////////////////////////
     -->

    <rdf:Description rdf:about="http://baleen.dstl.gov.uk/Relation">
        <rdfs:comment xml:lang="en">Records a relationship between named entities, explicitly mentioned within the source document.</rdfs:comment>
        <rdfs:comment xml:lang="en">A relationship between two entities</rdfs:comment>
    </rdf:Description>
    <rdf:Description rdf:about="http://baleen.dstl.gov.uk/source">
        <rdfs:comment xml:lang="en">The source of the relationship (subject)</rdfs:comment>
        <rdfs:comment xml:lang="en">The source of the relationship</rdfs:comment>
    </rdf:Description>
    <rdf:Description rdf:about="http://baleen.dstl.gov.uk/target">
        <rdfs:comment xml:lang="en">The target of the relationship</rdfs:comment>
        <rdfs:comment xml:lang="en">The target of the relationship (object)</rdfs:comment>
    </rdf:Description>
</rdf:RDF>



<!-- Generated by the OWL API (version 4.2.6.20160910-2108) https://github.com/owlcs/owlapi -->

